Computability/EvalString.lean
@@ -48,7 +48,7 @@ theorem evalc_prop_4: (use O c x).get h≤u ↔ (evalc O u c x).Dom :=
 
 
 -- the b2n $ n2b is to simplify later proofs where evals will be compared against _.
-def whatever := 999
+def whatever := 0
 noncomputable def evals (σ:List ℕ) (c:Code) (x:ℕ) := evalc (fun e=> b2n $ n2b $ σ.getD e whatever) σ.length c x
 
 end Nat.RecursiveIn.Code
